$\frac{1}{3+4i} = \frac{1}{3+4i} \frac{3+4i}{3+4i} = \frac{3+4i}{9+16i} =\frac{1}{5}(3-4i) \space | ausgeklammert$ 
$(1+i)⁴ = \left( \sqrt{2} + e^\frac{\pi}{4i} \right)$
$\ln\left( \frac{1}{1+i} \right) = -\ln(1+i)$
	    $=-\ln \sqrt{ 2}* e^\frac{\pi}{4i} = -\left( \ln \sqrt{ 2 } + \ln e^\frac{\pi}{4i} \right)$
		$=-\ln \sqrt{ 2 } - \frac{\pi}{4}i = -\frac{1}{2}\ln 2 - \frac{\pi}{i}i$


$$
\begin{align}
x_{1/2} &= \frac{-b \pm \sqrt{b^2 - 4ac}}{2a} \\
x_{1/2} &= \frac{-4 \pm \sqrt{4^2 - 4 \cdot 1 \cdot 8}}{2} \\
x_{1/2} &= \frac{-4 \pm \sqrt{16 - 32}}{2} \\
x_{1/2} &= \frac{-4 \pm \sqrt{-16}}{2} \\
x_{1/2} &= \frac{-4 \pm 4i}{2} \\
x_{1} &= -2 + 2i \\
x_{2} &= -2 - 2i
\end{align}
$$



$z = a+bi$
$\overline{z} = a-bi$
$z+\overline{z} = 2a$
$z-\overline{z}=2b$



$(x-x_{0})² + (y-y_{0})² = r²$
<<<<<<< HEAD
Kreis um $(x_{0}|y_{0})$ mit Radius r

$$
\begin{align*}

\end{align*}$$

=======
Kreis um $(x_{0}|y_{0})$ mit Radius r


$$
\begin{align*}
|z+1| &= \sqrt{ 2 } |z+1| \\
|a+bi+1| &= \sqrt{ 2 } (a+bi-1) \\
\sqrt{ (a+1)² +b²} &=\sqrt{ 2 } \sqrt{ (a-1)² +b²} \\
a²+2a+1+b² &= 2(a²-2a+1+b²) \\
0&=a²-6a+b²+1\\
0&=(a-3)²-9+b²+1\\
(a-3)²+b²&=8\\
\end{align*}
$$
